@prefix : <http://cognita.io/poderoEditor/layoutOntology/> .
@prefix owl:  <http://www.w3.org/2002/07/owl#>.
@prefix rdfs: <http://www.w3.org/2000/01/rdf-schema#>.
@prefix rdf:  <http://www.w3.org/1999/02/22-rdf-syntax-ns#>.
@prefix xsd:     <http://www.w3.org/2001/XMLSchema#>.
@prefix poder:         <http://poderopedia.com/vocab/> .
@prefix foaf: <http://xmlns.com/foaf/0.1/> .

: a owl:Ontology;
		rdfs:label "Layout Ontology" .


################
### CLASSES  ###
################

:FormView a owl:Class;
			rdfs:label "Class of a view." .

:VisualWidget a owl:Class;
			  rdfs:label "Class of all the visual widgets" .


:HTMLWidget rdfs:subClassOf :VisualWidget ;
			rdfs:label "Class of all the HTML Widgets" .

:HTMLInputTextWidget rdfs:subClassOf :HTMLWidget ;
					 rdfs:label "HTML Input text widget" .

:HTMLInputNumberWidget rdfs:subClassOf :HTMLWidget ;
					 rdfs:label "HTML Input number widget" .

:HTMLInputDateWidget rdfs:subClassOf :HTMLWidget ;
					 rdfs:label "HTML Input date widget" .

:HTMLTextareaWidget rdfs:subClassOf :HTMLWidget ;
					 rdfs:label "HTML textarea widget" .

:HTMLSelectionWidget rdfs:subClassOf :HTMLWidget ;
					 rdfs:label "HTML selection widgets" .

:HTMLRadioWidget rdfs:subClassOf :HTMLSelectionWidget ;
					 rdfs:label "HTML radio widget" .

:HTMLCheckboxWidget rdfs:subClassOf :HTMLSelectionWidget ;
					 rdfs:label "HTML checkbox widget" .

##################
### PREDICATES  ###
##################


:positionNumber a owl:DatatypeProperty;
			 rdfs:label "Order number";
			 rdfs:comment "Defines the priority in which a widget will be included on an element. The elements will be sorted based on this property to be displayed";
			 rdfs:domain :VisualWidget;
			 rdfs:range xsd:integer .

:anchoredTo a owl:ObjectProperty;
			rdfs:label "Anchored to";
			rdfs:comment "Defines an entity (e.g., canvas, DOM element) to which this widget should be anchored to.";
			rdfs:domain :VisualWidget .

:restrictionFunction a owl:DatatypeProperty;
					 rdfs:label "Restriction function";
					 rdfs:comment "Contains the name of a potential function that can be used to validate the input. This function can be a Javascript function for HTML documents or any other function in other contexts.";
					 rdfs:domain :HTMLWidget;
					 rdfs:range xsd:string .

:predicateDisplayed a owl:ObjectProperty;
			rdfs:label "Predicate displayed";
			rdfs:comment "Defines the predicate that will be displayed in the form.";
			rdfs:domain :VisualWidget .


:hasWidget a owl:ObjectProperty;
			rdfs:label "has widget";
			rdfs:comment "Relates this view with one or more widgets";
			rdfs:domain :FormView;
			rdfs:range :VisualWidget .


:classAssociated a owl:ObjectProperty;
			rdfs:label "Class associated";
			rdfs:comment "Class associated to a view";
			rdfs:domain :FormView ;
			rdfs:range owl:Class .

:hasSubView a owl:ObjectProperty;
			rdfs:label "Has subview";
			rdfs:comment "Subview associated to a view" ;
			rdfs:domain :FormView ;
			rdfs:range :FormView .

:viewRestriction a owl:ObjectProperty;
				rdfs:label "View Restriction" ;
				rdfs:comment "A property that defines potential restrictions to access a view" ;
				rdfs:domain :FormView .

:userViewRestriction a owl:ObjectProperty;
				rdfs:label "User View Restriction" ;
				rdfs:comment "A property that defines potential restrictions to access a view by users" ;
				rdfs:subPropertyOf :viewRestriction .
				rdfs:range foaf:Person .

:groupViewRestriction a owl:ObjectProperty;
				rdfs:label "Group View Restriction" ;
				rdfs:comment "A property that defines potential restrictions to access a view by groups" ;
				rdfs:subPropertyOf :viewRestriction ;
				rdfs:range foaf:Group .


#################
### EXAMPLES  ###
#################


<#basicView> a :FormView ;
			:classAssociated foaf:Person ;
			:hasWidget [ a :HTMLInputTextWidget, :HTMLWidget;
          				:predicateDisplayed foaf:firstName;
		  				:positionNumber 0;
		  				:anchoredTo "myForm" 
		  			   ],
		  			   [ a :HTMLInputTextWidget, :HTMLWidget;
		  				:predicateDisplayed foaf:familyName;
		  				:positionNumber 1;
		  				:anchoredTo "myForm" 
		  			   ],
		  			   [ a :HTMLInputCalendarWidget, :HTMLWidget;
		  				:predicateDisplayed foaf:birthday;
		  				:positionNumber 2;
		  				:anchoredTo "myForm" 
		  			   ],
		  			   [ a :HTMLResourceWidget, :HTMLWidget;
						   :predicateDisplayed poder:countryOfResidence ;
						   :positionNumber 3;
						   :anchoredTo "myForm"
					   ] ;
			:hasSubView [
						a :FormView ;
						:classAssociated poder:Marriage ;
						:hasWidget [ a :HTMLInputTextWidget;
									 :predicateDisplayed poder:connectionStartDate;
									 :positionNumber 1;
									 :anchoredTo "myForm"
								   ],
								   [ a :HTMLInputTextWidget;
									 :predicateDisplayed poder:connectionEndDate;
									 :positionNumber 2;
									 :anchoredTo "myForm"
								   ],
								   [ a :HTMLInputTextWidget;
									 :predicateDisplayed poder:hasSpouse;
									 :positionNumber 1;
									 :anchoredTo "myForm"
								   ]
						]

			]

